\documentclass[]{article}

\def\imp{\to} %implies instead of \to so it's easier to read in logic language
\def\ifof{\leftrightarrow} %if and only if (iff already exists)
\def\n{\neg}%easier to write
\usepackage{proof}
\usepackage{amssymb}

\title{Some Proof of Logic}
\author{}
\date{}

\begin{document}
\maketitle
\begin{enumerate}
	\item $\vdash_{INT}$ (A$\imp\neg$B)$\imp$(B$\imp\neg$A)
	$$ 
	\infer[^{i\imp (1)}]{(A\imp\neg B)\imp(B\imp\neg A)}{
	  \infer[^{i \imp (3)}]{B\imp\neg A}
	  {
	  	\infer[^{i\neg (2)}]{\neg A}
	  	{
	  	  \infer[^{i \bot}]{\bot}
	  	  {
	  	  	\infer[^{e\imp}]{\neg B, B}
	  	  	{
	  	  		\infer[^{(1)}]{A\imp\neg B}{}, & \infer[^{(2)}]{A}{}
	  	  	}
	  	  }
	  	}
	  }
	} 
	$$
	\item $\vdash_{INT}$ A $\imp\neg\neg$A 
	$$
	\infer[^{i\imp(1)}]{A\imp\neg\neg A}{
	  \infer[^{i\neg(2)}]{\neg\neg A}{
	  	\infer[i \bot]{\bot}{\infer[^{(1)}]{A}{},\infer[^{(2)}]{\neg A}{}}
	  }
	}
	$$

	$\nvdash_{INT} \neg\neg A \imp A$ but $\nvdash_{CL} \neg\neg A \imp A$
	$$
	\infer[^{i\imp(1)}]{\neg\neg A \imp A}{
	  \infer[^{e\neg(2) \gets \textrm{Problem for INT}}]{A}{
	    \infer[^{i\bot}]{\bot}{\infer[^{(1)}]{\neg\neg A}{},\infer[^{(2)}]{\neg A}{}}
  	  }
	}
	$$
	
	\item 49.b $\vdash_{INT} \neg \neg \neg A \ifof \neg A$
	
	$\vdash \neg A \imp \neg \neg \neg A$
	$$
	\infer[^{i\imp(1)}]{\neg A \imp \neg \n\n A}{
	  \infer[^{i\n(2)}]{\n\n\n A}{
	    \infer[^{i\bot}]{\bot}{
	      \infer[^{(1)}]{\n A}{}, \infer[^{(2)}]{\n\n A}{}	
	    }
	  }
	}
	$$
	
	$\vdash \n\n\n A \imp \neg A$
	$$
	\infer[^{i\imp (2)}]{\n\n\n A \imp \neg A}{
	  \infer[^{i\n(1)}]{\n A}{
	    \infer[^{i\bot}]{\bot}{
	      \infer[^{RD \textrm{ (ex. 2)}}]{\n\n A}{\infer[^{(1)}]{A}{}} & \infer[^{(2)}]{\n\n\n A}{} 
	    }	
	  }	
	}
	$$
	\pagebreak
	\item 50 a. $\n(A\ifof \n A)$
	$$
	\infer[^{i\n (1)}]{\n(A\ifof \n A)}{
	  \infer[^{i \bot}]{\bot}{
	    \infer[^{i\n (2)}]{\n A}{
	    	\infer[^{i \bot}]{\bot}{
	    	  \infer[^{e \imp}]{\n A, A}{
	    	  	\infer[^{e \land}]{A \imp \n A}
	    	  		{\infer[^{(1)}]{(A \imp \n A) \land (A \gets \n A)}{}}{}
	    	  		&
	    	  		\infer[^{(2)}]{A}{}
    		  }
	    	}
    	}
	    &
	    \infer[^{e \imp}]{A}{
	    \infer[^{i\n (2)}]{\n A}{
	    	\infer[^{i \bot}]{\bot}{
	    		\infer[^{e \imp}]{\n A, A}{
	    			\infer[^{e \land}]{A \imp \n A}
	    			{\infer[^{(1)}]{(A \imp \n A) \land (A \gets \n A)}{}}{}
	    			&
	    			\infer[^{(2)}]{A}{}
	    		}
	    	}
	    }
	    &
	    \infer[^{(1)}]{\n A \imp A}{}
        }	
	  }
	}
	$$
	
	\item 63. De Morgan: $\n(A\lor B) \ifof \n A \land \n B$
	
	$\gets$
	$$
	\infer[^{i \imp (1)}]{(\n A  \land \n B) \imp \n (A \lor B)}{
	  \infer[^{i \n (2)}]{\n (A \lor B)}{
	    \infer[^{e \lor (3)(4)}]{\bot}{
	    \infer[^{(2)}]{A\lor B}{}
	    &
	    \infer[^{i \bot}]{\bot}{
	      \infer[^{e \land}]{\neg A}{\infer[^{(1)}]{\neg A \land \n B}{}}
	      &
	      \infer[^{(3)}]{A}{}	
	    }
    	&
    	\infer[^{i \bot}]{\bot}{
    		\infer[^{e \land}]{\neg B}{\infer[^{(1)}]{\neg A \land \n B}{}}
    		&
    		\infer[^{(4)}]{B}{}	
    	}	
	    }	
	  }
	}
	$$
	$\imp$
	$$
	
	$$
\end{enumerate}

\end{document}